Revise Vale CreateHeaplets to take list of buffer_info

vale/code/arch/x64/Vale.X64.Memory.fsti
@@ -390,10 +390,9 @@ let buffer_info_disjoint (bi1 bi2:buffer_info) =
   loc_disjoint (loc_buffer bi1.bi_buffer) (loc_buffer bi2.bi_buffer)
 
 // Requirements for enabling heaplets
-let init_heaplets_req (h:vale_heap) (bs:Seq.seq buffer_info) (modloc:loc) =
+let init_heaplets_req (h:vale_heap) (bs:Seq.seq buffer_info) =
   (forall (i:nat).{:pattern (Seq.index bs i)} i < Seq.length bs ==>
-    buffer_readable h (Seq.index bs i).bi_buffer /\
-    ((Seq.index bs i).bi_mutable == Mutable ==> loc_includes modloc (loc_buffer (Seq.index bs i).bi_buffer))) /\
+    buffer_readable h (Seq.index bs i).bi_buffer) /\
   (forall (i1 i2:nat).{:pattern (Seq.index bs i1); (Seq.index bs i2)}
     i1 < Seq.length bs /\ i2 < Seq.length bs ==> buffer_info_disjoint (Seq.index bs i1) (Seq.index bs i2))
 
